LocallyNameless/Reduction.v
@@ -1,0 +1,467 @@
+From FormalSystems Require Export LocallyNameless.STLC.
+
+(** * Experiments with the definition of reduction *)
+
+(** ** Contraction *)
+
+Inductive Contraction : Tm -> Tm -> Prop :=
+| Contraction_Fun :
+  forall (t1 t2 : Tm),
+    lc (abs t1) ->
+    Value t2 ->
+    Contraction (app (abs t1) t2) (t1 {[ 0 ~> t2 ]}).
+
+#[export] Hint Constructors Contraction : core.
+
+Lemma lc_Contraction_l :
+  forall t t' : Tm,
+    Contraction t t' -> lc t.
+Proof.
+  intros t t'; destruct 1 as [t t' Hlc Hv].
+  constructor; [easy |].
+  now apply lc_Value.
+Qed.
+
+Lemma lc_Contraction_r :
+  forall t t' : Tm,
+    Contraction t t' -> lc t'.
+Proof.
+  intros t t'; destruct 1 as [t t' Hlc Hv].
+  apply lc_open; [easy |].
+  now apply lc_Value.
+Qed.
+
+(** ** A more modular definition *)
+
+Module modular.
+
+Inductive Step' : Tm -> Tm -> Prop :=
+| Step'_Contraction :
+  forall t t' : Tm,
+    Contraction t t' ->
+    Step' t t'
+| Step'_FunCongrL :
+  forall (t1 t1' t2 : Tm),
+    lc t2 ->
+    Step' t1 t1' ->
+    Step' (app t1 t2) (app t1' t2)
+| Step'_FunCongrR :
+  forall (t1 t2 t2' : Tm),
+    Value t1 ->
+    Step' t2 t2' ->
+    Step' (app t1 t2) (app t1 t2').
+
+#[export] Hint Constructors Step' : core.
+
+Lemma Step'_spec :
+  forall t t' : Tm,
+    Step' t t' <-> Step t t'.
+Proof.
+  split.
+  - induction 1.
+    + destruct H.
+      now constructor.
+    + now constructor.
+    + now constructor.
+  - induction 1.
+    + now constructor.
+    + now constructor 2.
+    + now constructor 3.
+Qed.
+
+Lemma lc_Step'_l :
+  forall t t' : Tm,
+    Step' t t' -> lc t.
+Proof.
+  induction 1.
+  - now apply lc_Contraction_l in H.
+  - now constructor.
+  - constructor; [| easy ].
+    now apply lc_Value.
+Qed.
+
+Lemma lc_Step'_r :
+  forall t t' : Tm,
+    Step' t t' -> lc t'.
+Proof.
+  induction 1.
+  - now apply lc_Contraction_r in H.
+  - now constructor.
+  - constructor; [| easy ].
+    now apply lc_Value.
+Qed.
+
+Lemma preservation :
+  forall (Γ : Ctx) (t1 t2 : Tm) (A : Ty),
+    Step t1 t2 ->
+    Typing Γ t1 A ->
+    Typing Γ t2 A.
+Proof.
+  intros * Hs Ht; revert t2 Hs.
+  induction Ht; intros; inversion Hs; subst.
+  - inversion Ht1; subst.
+    rewrite open'_spec with (x := fresh (l ++ fv t3)) by solve_fresh.
+    apply Typing_subst with A; [| easy].
+    apply Hcof.
+    now solve_fresh.
+  - now econstructor; eauto.
+  - now econstructor; eauto.
+Qed.
+
+Lemma progress :
+  forall (t : Tm) (A : Ty),
+    Typing [] t A ->
+      Value t \/ exists t' : Tm, Step t t'.
+Proof.
+  intros t A Ht.
+  remember [] as Γ.
+  induction Ht; subst.
+  - now inversion H0.
+  - left; constructor.
+    apply lc_abs with l; intros x Hx.
+    now eapply lc_Typing, Hcof.
+  - destruct (IHHt1 eq_refl) as [ [t1' Hlc1] | [t1' Hs1] ].
+    + now destruct (IHHt2 eq_refl) as [ [t2' Hlc2] | [t2' Hs2] ]; eauto.
+    + now apply lc_Typing in Ht2; eauto.
+Qed.
+
+End modular.
+
+(** ** Definitions based on evaluation contexts *)
+
+Inductive EvalCtx : Type :=
+| Hole : EvalCtx
+| FunCongrL :
+  forall (E : EvalCtx) (t2 : Tm) (Hlc2 : lc t2), EvalCtx
+| FunCongrR :
+  forall (t1 : Tm) (v1 : Value t1) (E : EvalCtx), EvalCtx.
+
+Fixpoint plug (E : EvalCtx) (t : Tm) : Tm :=
+match E with
+| Hole => t
+| FunCongrL E' t2 _ => app (plug E' t) t2
+| FunCongrR t1 _ E' => app t1 (plug E' t)
+end.
+
+Lemma plug_Hole :
+  forall t : Tm,
+    plug Hole t = t.
+Proof.
+  easy.
+Qed.
+
+Lemma preservation_Contraction :
+  forall (Γ : Ctx) (t t' : Tm) (A : Ty),
+    Contraction t t' ->
+    Typing Γ t A ->
+    Typing Γ t' A.
+Proof.
+  induction 1; inversion 1; subst.
+  inversion H5; subst.
+  rewrite open'_spec with (x := fresh (l ++ fv t1)) by solve_fresh.
+  apply Typing_subst with A0; [| easy].
+  apply Hcof.
+  now solve_fresh.
+Qed.
+
+(** *** Definition of reduction as an inductive type *)
+
+Module inductive.
+
+Inductive Step' : Tm -> Tm -> Prop :=
+| mkStep' :
+  forall (E : EvalCtx) (t t' : Tm),
+    Contraction t t' -> Step' (plug E t) (plug E t').
+
+#[export] Hint Constructors Step' : core.
+
+Lemma Step'_spec :
+  forall t t' : Tm,
+    Step' t t' <-> Step t t'.
+Proof.
+  split.
+  - destruct 1 as [E t t' [] ].
+    induction E; cbn; intros.
+    + now constructor.
+    + now constructor; [| apply IHE].
+    + now constructor; [| apply IHE].
+  - induction 1.
+    + now apply (mkStep' Hole _ (t1 {{ 0 ~> t2 }})).
+    + destruct IHStep as [E u u' HC].
+      now apply (mkStep' (FunCongrL E t2 H)).
+    + destruct IHStep as [E u u' HC].
+      now apply (mkStep' (FunCongrR t1 H E)).
+Qed.
+
+Lemma lc_Step'_l :
+  forall t t' : Tm,
+    Step' t t' -> lc t.
+Proof.
+  intros t t'; destruct 1 as [E t t' Hc].
+  induction E; cbn.
+  - now apply lc_Contraction_l in Hc.
+  - now constructor.
+  - constructor; [| easy].
+    now apply lc_Value.
+Qed.
+
+Lemma lc_Step'_r :
+  forall t t' : Tm,
+    Step' t t' -> lc t'.
+Proof.
+  intros t t'; destruct 1 as [E t t' Hc].
+  induction E; cbn.
+  - now apply lc_Contraction_r in Hc.
+  - now constructor.
+  - constructor; [| easy].
+    now apply lc_Value.
+Qed.
+
+Lemma preservation :
+  forall (Γ : Ctx) (t t' : Tm) (A : Ty),
+    Step' t t' ->
+    Typing Γ t A ->
+    Typing Γ t' A.
+Proof.
+  intros Γ t t' A; destruct 1 as [E t t' Hc].
+  revert A.
+  induction E; cbn; intros.
+  - now eapply preservation_Contraction; eauto.
+  - now inversion H; subst; econstructor; eauto.
+  - now inversion H; subst; econstructor; eauto.
+Qed.
+
+Lemma progress :
+  forall (t : Tm) (A : Ty),
+    Typing [] t A ->
+      Value t \/ exists t' : Tm, Step' t t'.
+Proof.
+  intros t A Ht.
+  remember [] as Γ.
+  induction Ht; subst.
+  - now inversion H0.
+  - left; constructor.
+    apply lc_abs with l.
+    intros x Hx.
+    now eapply lc_Typing, Hcof.
+  - destruct (IHHt1 eq_refl) as [ [t1' Hlc1] | [t1' Hs1] ].
+    + destruct (IHHt2 eq_refl) as [ [t2' Hlc2] | [t2' Hs2] ].
+      * right.
+        exists (plug Hole (t1' {[ 0 ~> abs t2' ]})).
+        now rewrite <- plug_Hole at 1.
+      * right.
+        destruct Hs2 as [E t2 t2' Hc].
+        exists (plug (FunCongrR (abs t1') ltac:(easy) E) t2').
+        change (app (abs t1') (plug E t2)) with (plug (FunCongrR (abs t1') ltac:(easy) E) t2).
+        easy.
+    + destruct Hs1 as [E t1 t1' Hc].
+      apply lc_Typing in Ht2.
+      right.
+      exists (plug (FunCongrL E t2 Ht2) t1').
+      change (app (plug E t1) t2) with (plug (FunCongrL E t2 Ht2) t1).
+      easy.
+Qed.
+
+End inductive.
+
+(** *** Definition of reduction with an existential quantifier *)
+
+Module ex.
+
+Definition Step' (t t' : Tm) : Prop :=
+  exists (E : EvalCtx) (u u' : Tm),
+    t = plug E u /\
+    t' = plug E u' /\
+    Contraction u u'.
+
+Lemma Step'_spec :
+  forall t t' : Tm,
+    Step' t t' <-> Step t t'.
+Proof.
+  split.
+  - intros (E & u & u' & -> & -> & []); clear u u'.
+    induction E; cbn; intros.
+    + now constructor.
+    + now constructor; [| apply IHE].
+    + now constructor; [| apply IHE].
+  - induction 1.
+    + exists Hole.
+      now do 2 eexists.
+    + destruct IHStep as (E & u & u' & -> & -> & HC).
+      exists (FunCongrL E t2 H).
+      now do 2 eexists.
+    + destruct IHStep as (E & u & u' & -> & -> & HC).
+      exists (FunCongrR t1 H E).
+      now do 2 eexists.
+Qed.
+
+Lemma lc_Step'_l :
+  forall t t' : Tm,
+    Step' t t' -> lc t.
+Proof.
+  intros ? ? (E & t & t' & -> & -> & Hc).
+  induction E; cbn.
+  - now apply lc_Contraction_l in Hc.
+  - now constructor.
+  - constructor; [| easy].
+    now apply lc_Value.
+Qed.
+
+Lemma lc_Step'_r :
+  forall t t' : Tm,
+    Step' t t' -> lc t'.
+Proof.
+  intros ? ? (E & t & t' & -> & -> & Hc).
+  induction E; cbn.
+  - now apply lc_Contraction_r in Hc.
+  - now constructor.
+  - constructor; [| easy].
+    now apply lc_Value.
+Qed.
+
+Lemma preservation :
+  forall (Γ : Ctx) (t t' : Tm) (A : Ty),
+    Step' t t' ->
+    Typing Γ t A ->
+    Typing Γ t' A.
+Proof.
+  intros * (E & u & u' & -> & -> & HC).
+  revert A.
+  induction E; cbn; intros.
+  - now eapply preservation_Contraction; eauto.
+  - now inversion H; subst; econstructor; eauto.
+  - now inversion H; subst; econstructor; eauto.
+Qed.
+
+Lemma progress :
+  forall (t : Tm) (A : Ty),
+    Typing [] t A ->
+      Value t \/ exists t' : Tm, Step' t t'.
+Proof.
+  intros t A Ht.
+  remember [] as Γ.
+  induction Ht; subst.
+  - now inversion H0.
+  - left; constructor.
+    apply lc_abs with l.
+    intros x Hx.
+    now eapply lc_Typing, Hcof.
+  - destruct (IHHt1 eq_refl) as [ [t1' Hlc1] | [t1' Hs1] ].
+    + destruct (IHHt2 eq_refl) as [ [t2' Hlc2] | [t2' Hs2] ].
+      * right; unfold Step'.
+        exists (t1' {[ 0 ~> abs t2' ]}).
+        now exists Hole, (app (abs t1') (abs t2')), (t1' {[ 0 ~> abs t2' ]}); cbn.
+      * right; unfold Step'.
+        destruct Hs2 as (E & u & u' & -> & -> & Hc).
+        now exists
+          (plug (FunCongrR (abs t1') ltac:(easy) E) u'),
+          (FunCongrR (abs t1') ltac:(easy) E),
+          u, u'; cbn.
+    + destruct Hs1 as (E & u & u' & -> & -> & Hc).
+      apply lc_Typing in Ht2.
+      right; unfold Step'.
+      now exists (plug (FunCongrL E t2 Ht2) u'), (FunCongrL E t2 Ht2), u, u'; cbn.
+Qed.
+
+End ex.
+
+(** *** Definition of reduction as a record *)
+
+Module record.
+
+Record Step' (t t' : Tm) : Prop := mkStep'
+{
+  E : EvalCtx;
+  u : Tm;
+  u' : Tm;
+  Ht : t = plug E u;
+  Ht' : t' = plug E u';
+  HC : Contraction u u';
+}.
+
+Lemma Step'_spec :
+  forall t t' : Tm,
+    Step' t t' <-> Step t t'.
+Proof.
+  split.
+  - intros [E u u' -> -> [] ].
+    induction E; cbn; intros.
+    + now constructor.
+    + now constructor; [| apply IHE].
+    + now constructor; [| apply IHE].
+  - induction 1.
+    + now eapply (mkStep' _ _ Hole).
+    + destruct IHStep as [E u u' -> -> HC].
+      now eapply (mkStep' _ _ (FunCongrL E t2 H)).
+    + destruct IHStep as [E u u' -> -> HC].
+      now eapply (mkStep' _ _ (FunCongrR t1 H E)).
+Qed.
+
+Lemma lc_Step'_l :
+  forall t t' : Tm,
+    Step' t t' -> lc t.
+Proof.
+  intros ? ? [E t t' -> -> Hc].
+  induction E; cbn.
+  - now apply lc_Contraction_l in Hc.
+  - now constructor.
+  - constructor; [| easy].
+    now apply lc_Value.
+Qed.
+
+Lemma lc_Step'_r :
+  forall t t' : Tm,
+    Step' t t' -> lc t'.
+Proof.
+  intros ? ? [E t t' -> -> Hc].
+  induction E; cbn.
+  - now apply lc_Contraction_r in Hc.
+  - now constructor.
+  - constructor; [| easy].
+    now apply lc_Value.
+Qed.
+
+Lemma preservation :
+  forall (Γ : Ctx) (t t' : Tm) (A : Ty),
+    Step' t t' ->
+    Typing Γ t A ->
+    Typing Γ t' A.
+Proof.
+  intros * [E t t' -> -> Hc].
+  revert A.
+  induction E; cbn; intros.
+  - now eapply preservation_Contraction; eauto.
+  - now inversion H; subst; econstructor; eauto.
+  - now inversion H; subst; econstructor; eauto.
+Qed.
+
+Lemma progress :
+  forall (t : Tm) (A : Ty),
+    Typing [] t A ->
+      Value t \/ exists t' : Tm, Step' t t'.
+Proof.
+  intros t A Ht.
+  remember [] as Γ.
+  induction Ht; subst.
+  - now inversion H0.
+  - left; constructor.
+    apply lc_abs with l.
+    intros x Hx.
+    now eapply lc_Typing, Hcof.
+  - destruct (IHHt1 eq_refl) as [ [t1' Hlc1] | [t1' Hs1] ].
+    + destruct (IHHt2 eq_refl) as [ [t2' Hlc2] | [t2' Hs2] ].
+      * right.
+        exists (t1' {[ 0 ~> abs t2' ]}).
+        now eapply (mkStep' _ _ Hole (app (abs t1') (abs t2'))); cbn; eauto.
+      * right.
+        destruct Hs2 as [E u u' -> -> Hc].
+        exists (app (abs t1') (plug E u')).
+        now eapply (mkStep' _ _ (FunCongrR (abs t1') ltac:(easy) E)); cbn; eauto.
+    + destruct Hs1 as [E u u' -> -> Hc].
+      apply lc_Typing in Ht2.
+      right.
+      exists (app (plug E u') t2).
+      now eapply (mkStep' _ _ (FunCongrL E t2 Ht2)); cbn; eauto.
+Qed.
+
+End record.
